src/proofs/no_slashable_attestations/supporting_lemmas/dv_next_preserves_ind_inv/ind_inv_dv_next.dfy
@@ -97,8 +97,8 @@ module Ind_Inv_DV_Next
     ensures invs_group_5(dv')
     {
         lem_inv_att_slashing_db_hist_keeps_track_of_only_rcvd_att_duties_dv_next(dv, e, dv');    
-        lem_inv_exists_db_in_att_slashing_db_hist_for_every_validity_pred_dv_next(dv, e, dv');  
-        lem_inv_validity_pred_for_slot_k_is_stored_in_att_slashing_db_hist_k_dv_next(dv, e, dv');          
+        lem_inv_exists_db_in_att_slashing_db_hist_and_duty_for_every_validity_predicate_dv_next(dv, e, dv');  
+        lem_inv_current_validity_predicate_for_slot_k_is_stored_in_att_slashing_db_hist_k_dv_next(dv, e, dv');          
     }
 
     lemma lem_ind_inv_dv_next_invs_group_6(dv: DVState, e: DV.Event, dv': DVState)       
@@ -137,7 +137,7 @@ module Ind_Inv_DV_Next
     lemma lem_ind_inv_implies_intermediate_steps_helper_2(dv: DVState)
     requires ind_inv(dv)  
     ensures inv_sent_vp_is_based_on_existing_slashing_db_and_rcvd_att_duty(dv)
-    ensures inv_joined_consensus_instances_implied_the_delivery_of_att_duties(dv)   
+    ensures inv_active_consensus_instances_implied_the_delivery_of_att_duties(dv)   
     ensures same_honest_nodes_in_dv_and_ci(dv)    
     ensures construct_signed_attestation_signature_assumptions_helper(
                 dv.construct_signed_attestation_signature,
@@ -145,7 +145,7 @@ module Ind_Inv_DV_Next
                 dv.all_nodes)  
     {    
         lem_inv_sent_vp_is_based_on_existing_slashing_db_and_rcvd_att_duty_ind_inv(dv);
-        lem_inv_joined_consensus_instances_implied_the_delivery_of_att_duties_ind_inv(dv);
+        lem_inv_active_consensus_instances_implied_the_delivery_of_att_duties_ind_inv(dv);
         lem_inv_queued_att_duty_is_rcvd_duty3_ind_inv(dv);      
         lem_construct_signed_attestation_signature_assumptions_helper(dv);       
     }
@@ -177,7 +177,7 @@ module Ind_Inv_DV_Next
     ensures inv_att_duty_in_next_delivery_is_not_lower_than_latest_served_att_duty(dv)
     ensures inv_att_duty_in_next_delivery_is_not_lower_than_rcvd_att_duties(dv)
     ensures inv_sent_vp_is_based_on_existing_slashing_db_and_rcvd_att_duty(dv)
-    ensures inv_joined_consensus_instances_implied_the_delivery_of_att_duties(dv)   
+    ensures inv_active_consensus_instances_implied_the_delivery_of_att_duties(dv)   
     ensures same_honest_nodes_in_dv_and_ci(dv)    
     ensures construct_signed_attestation_signature_assumptions_helper(
                 dv.construct_signed_attestation_signature,
@@ -201,7 +201,7 @@ module Ind_Inv_DV_Next
     requires ind_inv(dv)
     ensures inv_all_validity_predicates_are_stored_in_att_slashing_db_hist(dv')
     {
-        lem_inv_validity_pred_for_slot_k_is_stored_in_att_slashing_db_hist_k_inv_active_attestation_consensus_instances_predicate_is_in_att_slashing_db_hist(dv);
+        lem_inv_current_validity_predicate_for_slot_k_is_stored_in_att_slashing_db_hist_k_inv_active_attestation_consensus_instances_predicate_is_in_att_slashing_db_hist(dv);
         assert inv_active_attestation_consensus_instances_predicate_is_in_att_slashing_db_hist(dv);
 
         lem_inv_active_attestation_consensus_instances_keys_is_subset_of_att_slashing_db_hist(dv);
@@ -215,7 +215,7 @@ module Ind_Inv_DV_Next
                && inv_quorum_constraints(dv)
                && same_honest_nodes_in_dv_and_ci(dv)
                && inv_only_dv_construct_signed_attestation_signature(dv)    
-               && inv_sent_validity_predicate_only_for_slots_stored_in_att_slashing_db_hist_helper(dv)  
+               && inv_slots_for_sent_validity_predicate_are_stored_in_att_slashing_db_hist(dv)  
                && inv_active_attestation_consensus_instances_keys_is_subset_of_att_slashing_db_hist(dv)
                && inv_active_attestation_consensus_instances_predicate_is_in_att_slashing_db_hist(dv)
                ;
